code/bignum/Hacl.Bignum.AlmostMontgomery.fst
@@ -1,0 +1,102 @@
+module Hacl.Bignum.AlmostMontgomery
+
+open FStar.HyperStack
+open FStar.HyperStack.ST
+open FStar.Mul
+
+open Lib.IntTypes
+open Lib.Buffer
+
+open Hacl.Bignum.Definitions
+open Hacl.Bignum.Base
+open Hacl.Impl.Lib
+
+module ST = FStar.HyperStack.ST
+module Loops = Lib.LoopCombinators
+module LSeq = Lib.Sequence
+module B = LowStar.Buffer
+
+module S = Hacl.Spec.Bignum.AlmostMontgomery
+module SB = Hacl.Spec.Bignum
+module BN = Hacl.Bignum
+module BM = Hacl.Bignum.Montgomery
+
+friend Hacl.Spec.Bignum.AlmostMontgomery
+friend Hacl.Bignum.Montgomery
+
+#reset-options "--z3rlimit 50 --fuel 0 --ifuel 0"
+
+let bn_almost_mont_reduction #t k n nInv c res =
+  [@inline_let] let len = k.BN.len in
+  push_frame ();
+  let c0 = BM.bn_mont_reduction_loop_div_r #t k n nInv c res in
+  let tmp = create len (uint #t #SEC 0) in
+  let c1 = k.BN.sub res n tmp in
+  map2T len res (mask_select (uint #t 0 -. c0)) tmp res;
+  pop_frame ()
+
+
+let bn_almost_mont_mul #t k almost_mont_reduction n nInv_u64 aM bM resM =
+  [@inline_let] let len = k.BN.len in
+  push_frame ();
+  let c = create (len +! len) (uint #t 0) in
+  k.BN.mul aM bM c;
+  almost_mont_reduction n nInv_u64 c resM;
+  pop_frame ()
+
+
+let bn_almost_mont_sqr #t k almost_mont_reduction n nInv_u64 aM resM =
+  [@inline_let] let len = k.BN.len in
+  push_frame ();
+  let c = create (len +! len) (uint #t 0) in
+  k.BN.sqr aM c;
+  almost_mont_reduction n nInv_u64 c resM;
+  pop_frame ()
+
+
+let bn_almost_mont_reduction_u32 (len:BN.meta_len U32) : bn_almost_mont_reduction_st U32 len =
+  bn_almost_mont_reduction (BN.mk_runtime_bn U32 len)
+let bn_almost_mont_mul_u32 (len:BN.meta_len U32) : bn_almost_mont_mul_st U32 len =
+  bn_almost_mont_mul (BN.mk_runtime_bn U32 len) (bn_almost_mont_reduction_u32 len)
+let bn_almost_mont_sqr_u32 (len:BN.meta_len U32) : bn_almost_mont_sqr_st U32 len =
+  bn_almost_mont_sqr (BN.mk_runtime_bn U32 len) (bn_almost_mont_reduction_u32 len)
+
+inline_for_extraction noextract
+let mk_runtime_almost_mont_u32 (len:BN.meta_len U32) : almost_mont U32 = {
+  bn = BN.mk_runtime_bn U32 len;
+  mont_check = BM.bn_check_modulus_u32 len;
+  precomp = BM.bn_precomp_r2_mod_n_u32 len;
+  reduction = bn_almost_mont_reduction_u32 len;
+  to = BM.bn_to_mont_u32 len;
+  from = BM.bn_from_mont_u32 len;
+  mul = bn_almost_mont_mul_u32 len;
+  sqr = bn_almost_mont_sqr_u32 len;
+}
+
+
+let bn_almost_mont_reduction_u64 (len:BN.meta_len U64) : bn_almost_mont_reduction_st U64 len =
+  bn_almost_mont_reduction (BN.mk_runtime_bn U64 len)
+let bn_almost_mont_mul_u64 (len:BN.meta_len U64) : bn_almost_mont_mul_st U64 len =
+  bn_almost_mont_mul (BN.mk_runtime_bn U64 len) (bn_almost_mont_reduction_u64 len)
+let bn_almost_mont_sqr_u64 (len:BN.meta_len U64) : bn_almost_mont_sqr_st U64 len =
+  bn_almost_mont_sqr (BN.mk_runtime_bn U64 len) (bn_almost_mont_reduction_u64 len)
+
+inline_for_extraction noextract
+let mk_runtime_almost_mont_u64 (len:BN.meta_len U64) : almost_mont U64 = {
+  bn = BN.mk_runtime_bn U64 len;
+  mont_check = BM.bn_check_modulus_u64 len;
+  precomp = BM.bn_precomp_r2_mod_n_u64 len;
+  reduction = bn_almost_mont_reduction_u64 len;
+  to = BM.bn_to_mont_u64 len;
+  from = BM.bn_from_mont_u64 len;
+  mul = bn_almost_mont_mul_u64 len;
+  sqr = bn_almost_mont_sqr_u64 len;
+}
+
+
+let mk_runtime_almost_mont (#t:limb_t) (len:BN.meta_len t) : almost_mont t =
+  match t with
+  | U32 -> mk_runtime_almost_mont_u32 len
+  | U64 -> mk_runtime_almost_mont_u64 len
+
+let mk_runtime_almost_mont_len_lemma #t len = ()
