code/bignum/Hacl.Spec.AlmostMontgomery.Lemmas.fst
@@ -1,0 +1,129 @@
+module Hacl.Spec.AlmostMontgomery.Lemmas
+
+open FStar.Mul
+
+open Lib.IntTypes
+open Lib.LoopCombinators
+
+module M = Hacl.Spec.Montgomery.Lemmas
+
+#reset-options "--z3rlimit 50 --fuel 0 --ifuel 0"
+
+///  High-level specification of Almost Montgomery Multiplication
+
+val almost_mont_reduction: pbits:pos -> rLen:nat -> n:pos -> mu:nat -> c:nat -> int
+let almost_mont_reduction pbits rLen n mu c =
+  let res = M.mont_reduction_loop_div_r pbits rLen n mu c in
+  if res < pow2 (pbits * rLen) then res else res - n
+
+val almost_mont_mul: pbits:pos -> rLen:nat -> n:pos -> mu:nat -> a:nat -> b:nat -> int
+let almost_mont_mul pbits rLen n mu a b =
+  let c = a * b in
+  almost_mont_reduction pbits rLen n mu c
+
+val almost_mont_sqr: pbits:pos -> rLen:nat -> n:pos -> mu:nat -> a:nat -> int
+let almost_mont_sqr pbits rLen n mu a =
+  let c = a * a in
+  almost_mont_reduction pbits rLen n mu c
+
+
+///  Lemma (almost_mont_mul pbits rLen n mu a b % n == a * b * d % n)
+
+val lemma_fits_c_lt_rr: c:nat -> r:pos -> n:pos -> Lemma
+  (requires c < r * r)
+  (ensures (c - n) / r < r)
+
+let lemma_fits_c_lt_rr c r n =
+  assert (c < r * r);
+  Math.Lemmas.cancel_mul_div r r;
+  assert (c / r < r);
+  Math.Lemmas.lemma_div_le (c - n) c r
+
+
+val almost_mont_reduction_lemma: pbits:pos -> rLen:nat -> n:pos -> d:int -> mu:nat -> c:nat -> Lemma
+  (requires (let r = pow2 (pbits * rLen) in
+    (1 + n * mu) % pow2 pbits == 0 /\ r * d % n == 1 /\ c < r * r))
+  (ensures  (let res = almost_mont_reduction pbits rLen n mu c in
+    let r = pow2 (pbits * rLen) in
+    res % n == c * d % n /\ res < r))
+
+let almost_mont_reduction_lemma pbits rLen n d mu c =
+  let r = pow2 (pbits * rLen) in
+  let res = M.mont_reduction_loop_div_r pbits rLen n mu c in
+  M.mont_reduction_loop_div_r_lemma pbits rLen n d mu c;
+  assert (res % n == c * d % n /\ res <= (c - n) / r + n);
+
+  let res1 = if res < r then res else res - n in
+  if res < r then ()
+  else begin
+    assert (res1 % n == (res - n) % n);
+    Math.Lemmas.lemma_mod_sub res n 1;
+    assert (res1 % n == res % n);
+    assert (res1 <= (c - n) / r);
+    lemma_fits_c_lt_rr c r n end
+
+
+val almost_mont_mul_lemma: pbits:pos -> rLen:nat -> n:pos -> d:int-> mu:nat -> a:nat -> b:nat -> Lemma
+  (requires (let r = pow2 (pbits * rLen) in
+    (1 + n * mu) % pow2 pbits == 0 /\ r * d % n == 1 /\ a < r /\ b < r /\ n < r))
+  (ensures  (let res = almost_mont_mul pbits rLen n mu a b in
+    let r = pow2 (pbits * rLen) in
+    res % n == a * b * d % n /\ res < r))
+
+let almost_mont_mul_lemma pbits rLen n d mu a b =
+  let r = pow2 (pbits * rLen) in
+  let res = almost_mont_mul pbits rLen n mu a b in
+  Math.Lemmas.lemma_mult_lt_sqr a b r;
+  assert (a * b < r * r);
+  almost_mont_reduction_lemma pbits rLen n d mu (a * b)
+
+
+///  Properties
+
+val from_almost_mont_mul_lemma: pbits:pos -> rLen:pos -> n:pos -> mu:nat -> aM:nat -> bM:nat -> Lemma
+  (requires (let r = pow2 (pbits * rLen) in
+    M.mont_pre pbits rLen n mu /\ aM < r /\ bM < r))
+  (ensures
+   (let cM = almost_mont_mul pbits rLen n mu aM bM in
+    let c = M.from_mont pbits rLen n mu cM in
+    let a = M.from_mont pbits rLen n mu aM in
+    let b = M.from_mont pbits rLen n mu bM in
+    c == a * b % n))
+
+let from_almost_mont_mul_lemma pbits rLen n mu aM bM =
+  let r = pow2 (pbits * rLen) in
+  let d, _ = M.eea_pow2_odd (pbits * rLen) n in
+  M.mont_preconditions pbits rLen n mu;
+  assert (r * d % n == 1 /\ n < r /\ (1 + n * mu) % pow2 pbits == 0);
+
+  let cM = almost_mont_mul pbits rLen n mu aM bM in
+  let c = M.from_mont pbits rLen n mu cM in
+  let a = M.from_mont pbits rLen n mu aM in
+  let b = M.from_mont pbits rLen n mu bM in
+
+  almost_mont_mul_lemma pbits rLen n d mu aM bM;
+  //assert (cM % n == aM * bM * d % n);
+  M.from_mont_lemma pbits rLen n d mu cM;
+  //assert (c == cM * d % n);
+
+  calc (==) { //c
+    cM * d % n;
+    (==) { Math.Lemmas.lemma_mod_mul_distr_l cM d n }
+    (aM * bM * d % n) * d % n;
+    (==) { Math.Lemmas.lemma_mod_mul_distr_l (aM * bM * d) d n }
+    aM * bM * d * d % n;
+    (==) { Math.Lemmas.paren_mul_right aM bM d }
+    aM * (bM * d) * d % n;
+    (==) {
+      Math.Lemmas.paren_mul_right aM (bM * d) d;
+      Math.Lemmas.swap_mul (bM * d) d;
+      Math.Lemmas.paren_mul_right aM d (bM * d) }
+    aM * d * (bM * d) % n;
+    (==) { Math.Lemmas.lemma_mod_mul_distr_l (aM * d) (bM * d) n }
+    (aM * d % n) * (bM * d) % n;
+    (==) { Math.Lemmas.lemma_mod_mul_distr_r (aM * d % n) (bM * d) n }
+    (aM * d % n) * (bM * d % n) % n;
+    };
+
+  M.from_mont_lemma pbits rLen n d mu aM;
+  M.from_mont_lemma pbits rLen n d mu bM
